src/tls/MAC_SHA1.fst
@@ -1,8 +1,9 @@
-﻿(* Copyright (C) 2012--2015 Microsoft Research and INRIA *)
+﻿module MAC_SHA1
 
-#light "off"
-
-module MAC_SHA1
+open FStar.Heap
+open FStar.HyperHeap
+open FStar.Seq
+open FStar.SeqProperties // for e.g. found
 
 open Platform.Bytes
 open TLSConstants
@@ -10,38 +11,66 @@ open TLSInfo
 open Platform.Error
 open TLSError
 
-type text = bytes
-type tag = bytes
-type keyrepr = bytes
-type key = {k:keyrepr}
-
+// idealizing HMAC 
 // for concreteness; the rest of the module is parametric in a 
-let a = HMAC(CoreCrypto.SHA1) 
 
-#if ideal 
-// We maintain a table of MACed plaintexts
-type entry = id * text * tag
-let log:ref<list<entry>> =ref []
-let rec tmem (e:id) (t:text) (xs: list<entry>) = 
-  match xs with
-      [] -> false
-    | (e',t',m)::res when e = e' && t = t' -> true
-    | (e',t',m)::res -> tmem e t res
-#endif
+let a = HMAC CoreCrypto.SHA1
 
-let gen (ki:id) = {k= CoreCrypto.random (macKeySize(a))}
 
-let mac (ki:id) key t =
-    let m = HMAC.tls_mac a key.k t in
-    #if ideal 
-    // We log every authenticated texts, with their index and resulting tag
-    log := (ki, t, m)::!log;
-    #endif
-    m
 
-let verify (ki:id) key t m =
-    HMAC.tls_macVerify a key.k t m
-    #if ideal 
+type id = i:id { is_MACOnly i.aeAlg \/ is_MtE i.aeAlg }
+
+type text = bytes
+type tag (i:id) = bytes
+type keyrepr (i:id) = bytes
+type key (i:id) = keyrepr i
+
+type good (i:id) (b:bytes) // TBD in Encode?
+
+
+// we keep the tag in case we want to enforce tag authentication
+type entry (i:id) = | Entry: t:tag i -> p:bytes { good i p } -> entry i
+
+// readers and writers share the same state: a log of MACed messages
+type state (i:id) (rw:rw) = | State: 
+  #region:rid -> // the region of the *writer*
+  key: key i ->
+  log: rref region (seq (entry i)) -> 
+  state i rw
+                             
+private type writer i = s:state i Writer
+private type reader i = s:state i Reader
+
+let gen writer_parent i = 
+  let kv = CoreCrypto.random (macKeySize a) in 
+  let writer_r = new_region writer_parent in 
+  let log = ralloc writer_r Seq.createEmpty in 
+  State #i #Reader #writer_r kv log, 
+  State #i #Writer #writer_r kv log
+
+val mac: i:id -> wr:writer i -> p:bytes { good i p } -> ST (tag i) 
+  (requires (fun h0 -> True))
+  (ensures (fun h0 t h1 -> 
+    modifies (Set.singleton wr.region) h0 h1 /\ // skipping modifies rref, as the region contains only one ref
+    sel h1 wr.log = snoc (sel h0 wr.log) (Entry t p)))
+
+let mac i wr p =
+    admit(); //$ why?
+    let t : tag i = HMAC.tls_mac a wr.key p in
+    wr.log := snoc !wr.log (Entry #i t p); // We log every authenticated texts, with their index and resulting tag
+    t
+
+val matches: i:id -> p:text -> entry i -> Tot bool 
+let matches i p (Entry #i _ p') = p = p'
+
+val verify: i:id -> rd:reader i -> p:bytes -> t:tag i -> ST bool
+  (requires (fun h0 -> True))
+  (ensures (fun h0 b h1 -> 
+    h0 = h1 /\ 
+    (b ==> good i p)))
+
+let verify i rd p t =
+    HMAC.tls_macVerify a rd.key p t 
     // We use the log to correct any verification errors
-    && tmem ki t !log
-    #endif
+    && 
+    is_Some (seq_find (matches i p) !rd.log)
