src/tls/Range.fst
@@ -293,8 +293,8 @@ let rangeClass (i:id) (r:range) =
 let fragment_range: range = (0,max_TLSPlaintext_fragment_length)
 
 // for writers, we keep track of actual ranges
-// and require point ranges when padding is not available.
-type frange (i:id) = rg:range { Wider fragment_range rg /\ (is_AEAD i.aeAlg ==> fst rg = snd rg) }
+// and we require point ranges when padding is not available.
+type frange (i:id) = rg:range { Wider fragment_range rg /\ (lhae i.aeAlg || fst rg = snd rg) }
 
 // we don't need the index for point ranges (e.g. non-appdata traffic)
 type frange_any = rg:range { Wider fragment_range rg /\ fst rg = snd rg } 
